src/program_proof/tulip/invariance/execute_abort.v
@@ -1,0 +1,157 @@
+From Perennial.program_proof.tulip Require Import prelude.
+From Perennial.program_proof.tulip.invariance Require Import execute_common.
+
+Section execute_abort.
+  Context `{!tulip_ghostG Σ}.
+
+  Lemma replica_inv_execute_abort γ gid rid clog ilog ts :
+    let clog' := clog ++ [CmdAbort ts] in
+    Forall (λ nc, (nc.1 <= length clog)%nat) ilog ->
+    is_txn_log_lb γ gid clog' -∗
+    own_replica_clog_half γ rid clog -∗
+    own_replica_ilog_half γ rid ilog -∗
+    group_inv γ gid -∗
+    replica_inv γ gid rid ==∗
+    own_replica_clog_half γ rid clog' ∗
+    own_replica_ilog_half γ rid ilog ∗
+    group_inv γ gid ∗
+    replica_inv γ gid rid.
+  Proof.
+    iIntros (clog' Hpos) "#Hloglb Hclogprog Hilogprog Hgroup Hrp".
+    iAssert (⌜not_stuck (apply_cmds clog')⌝)%I as %Hns.
+    { do 2 iNamed "Hgroup".
+      iDestruct (txn_log_prefix with "Hlog Hloglb") as %Hprefix.
+      iPureIntro.
+      eapply apply_cmds_not_stuck; [apply Hprefix | by rewrite Hrsm].
+    }
+    iAssert (is_group_aborted γ gid ts)%I as "#Hgabtts".
+    { do 2 iNamed "Hgroup".
+      (* First, show that [ts] must have aborted after applying [clog']. *)
+      destruct (apply_cmds clog') as [cmp histmp |] eqn:Happly; last done.
+      assert (Habted : cmp !! ts = Some false).
+      { rewrite apply_cmds_snoc /= /apply_abort in Happly.
+        destruct (apply_cmds clog) as [cmpp histmpp |]; last done.
+        destruct (cmpp !! ts) eqn:Hcmpp.
+        { destruct b; first done.
+          by inv Happly.
+        }
+        inv Happly.
+        by rewrite lookup_insert.
+      }
+      (* Next, show that [ts] must have aborted after applying the latest log. *)
+      iDestruct (txn_log_prefix with "Hlog Hloglb") as %Hprefix.
+      pose proof (apply_cmds_mono_cm Hprefix Hrsm Happly) as Hincl.
+      pose proof (lookup_weaken _ _ _ _ Habted Hincl) as Habtedcm.
+      iDestruct (group_commit_witness with "Hcm") as "#Hgabt".
+      { apply Habtedcm. }
+      iFrame "Hgabt".
+    }
+    do 2 iNamed "Hrp".
+    (* Agreement on the consistent and inconsistent logs. *)
+    iDestruct (replica_clog_agree with "Hclogprog Hclog") as %->.
+    iDestruct (replica_ilog_agree with "Hilogprog Hilog") as %->.
+    (* Update the consistent log. *)
+    iMod (replica_clog_update clog' with "Hclogprog Hclog") as "[Hclogprog Hclog]".
+    rewrite /not_stuck apply_cmds_snoc /= in Hns.
+    set st := LocalState _ _ _ _ _ _ in Hrsm.
+    (* Re-establish the RSM predicate. This will compute to the right form along
+    the way in each branch. *)
+    assert (Hrsm' : execute_cmds (merge_clog_ilog clog' ilog) = execute_abort st ts).
+    { rewrite merge_clog_ilog_snoc_clog; last apply Hpos.
+      by rewrite execute_cmds_snoc Hrsm.
+    }
+    iFrame "Hclogprog Hilogprog Hgroup".
+    unshelve epose proof (execute_cmds_apply_cmds clog ilog cm histm _) as Happly.
+    { by eauto. }
+    rewrite /apply_abort Happly in Hns.
+    subst st.
+    rewrite /execute_abort in Hrsm'.
+    destruct (cm !! ts) as [b |] eqn:Hcm.
+    { (* Case: Txn [ts] already finalized. Contradiction for committed; no-op for aborted. *)
+      destruct b; first done.
+      by iFrame "∗ # %".
+    }
+    (* Case: Txn [ts] not finalized. *)
+    (* Obtain facts about domain of the timestamp maps. *)
+    pose proof (map_Forall2_dom_L _ _ _ Hlenkvd) as Hdomsptsm.
+    symmetry in Hdomsptsm. rewrite Hdomkvdm in Hdomsptsm.
+    pose proof (map_Forall2_dom_L _ _ _ Hsptsmlk) as Hdomptsm.
+    symmetry in Hdomptsm. rewrite Hdomsptsm in Hdomptsm.
+    destruct (cpm !! ts) as [pwrs |] eqn:Hcpm.
+    { (* Case: Txn [ts] prepared. *)
+      (* Set commit map to false, reset currently prepared map and release locks. *)
+      iDestruct (big_sepM_delete _ _ ts with "Hsafep") as "[Hpwrs Hsafep']".
+      { apply Hcpm. }
+      iAssert (⌜dom pwrs ⊆ keys_all⌝)%I as %Hdompwrs.
+      { iDestruct "Hpwrs" as (wrs) "(_ & _ & %Hvwrs & _ & %Hpwrs)".
+        iPureIntro.
+        rewrite Hpwrs wrs_group_keys_group_dom. set_solver.
+      }
+      set cpm' := delete _ cpm in Hrsm'.
+      set ptsm' := release _ ptsm in Hrsm'.
+      iAssert (group_aborted_if_validated γ gid kvdm histm ptsm')%I as "#Hgabt'".
+      { iIntros (k t).
+        destruct (decide (k ∈ dom pwrs)) as [Hin | Hnotin]; last first.
+        { by rewrite release_unmodified; last by apply not_elem_of_dom. }
+        assert (is_Some (kvdm !! k)) as [vl Hvl].
+        { rewrite -elem_of_dom Hdomkvdm. clear -Hin Hdompwrs. set_solver. }
+        pose proof (execute_cmds_dom_histm Hrsm) as Hdomhistm.
+        assert (is_Some (histm !! k)) as [h Hh].
+        { rewrite -elem_of_dom Hdomhistm. clear -Hin Hdompwrs. set_solver. }
+        rewrite release_modified; last first.
+        { rewrite Hdomptsm. clear -Hin Hdompwrs. set_solver. }
+        { apply Hin. }
+        rewrite Hvl Hh.
+        destruct (vl !! t) as [b |] eqn:Hvlt; last done.
+        destruct b; last done.
+        case_decide as Ht; last done.
+        destruct Ht as (Hgelen & Hnz).
+        assert (is_Some (ptsm !! k)) as [pts Hpts].
+        { rewrite -elem_of_dom Hdomptsm. clear -Hin Hdompwrs. set_solver. }
+        iSpecialize ("Hgabt" $! k t).
+        rewrite Hvl Hh Hpts Hvlt.
+        case_decide as Ht; first done.
+        apply Classical_Prop.not_and_or in Ht.
+        destruct Ht as [Hltlen | Ht].
+        { exfalso.
+          rewrite Nat.nle_gt in Hltlen.
+          clear -Hgelen Hltlen. lia.
+        }
+        apply dec_stable in Ht. subst t.
+        (* Prove that [k] must be locked by [ts] (i.e., [ts = pts]. *)
+        specialize (Hpil _ _ _ Hcpm Hin).
+        rewrite Hpil in Hpts. inv Hpts.
+        iFrame "Hgabtts".
+      }
+      iFrame "∗ # %".
+      iPureIntro.
+      split.
+      { rewrite dom_insert_L dom_delete_L. clear -Hvtss.
+        rewrite -union_assoc union_comm -union_assoc difference_union_L.
+        set_solver.
+      }
+      split.
+      { rewrite map_Forall2_forall.
+        split; last by rewrite release_dom Hdomsptsm Hdomptsm.
+        intros k spts pts Hspts Hpts Hnz.
+        destruct (decide (k ∈ dom pwrs)) as [Hin | Hnotin]; last first.
+        { rewrite release_unmodified in Hpts; last by apply not_elem_of_dom.
+          apply (map_Forall2_lookup_Some _ _ _ _ _ _ Hspts Hpts Hsptsmlk Hnz).
+        }
+        rewrite release_modified in Hpts; last first.
+        { rewrite Hdomptsm. clear -Hin Hdompwrs. set_solver. }
+        { apply Hin. }
+        inv Hpts.
+      }
+      split.
+      { by apply prepared_impl_locked_inv_release. }
+      { rewrite lookup_delete_None. by right. }
+    }
+    (* Case: Txn [ts] not prepared. Set commit map to false. *)
+    iFrame "∗ # %".
+    iPureIntro.
+    rewrite dom_insert_L.
+    clear -Hvtss. set_solver.
+  Qed.
+
+End execute_abort.
