src/program_proof/tulip/invariance/execute_commit.v
@@ -1,0 +1,198 @@
+From Perennial.program_proof.tulip Require Import prelude.
+From Perennial.program_proof.tulip.invariance Require Import execute_common.
+
+Section execute_commit.
+  Context `{!tulip_ghostG Σ}.
+
+  Lemma replica_inv_execute_commit γ gid rid clog ilog ts pwrs :
+    let clog' := clog ++ [CmdCommit ts pwrs] in
+    Forall (λ nc, (nc.1 <= length clog)%nat) ilog ->
+    is_txn_log_lb γ gid clog' -∗
+    own_replica_clog_half γ rid clog -∗
+    own_replica_ilog_half γ rid ilog -∗
+    group_inv γ gid -∗
+    replica_inv γ gid rid ==∗
+    own_replica_clog_half γ rid clog' ∗
+    own_replica_ilog_half γ rid ilog ∗
+    group_inv γ gid ∗
+    replica_inv γ gid rid.
+  Proof.
+    iIntros (clog' Hpos) "#Hloglb Hclogprog Hilogprog Hgroup Hrp".
+    iAssert (⌜not_stuck (apply_cmds clog')⌝)%I as %Hns.
+    { do 2 iNamed "Hgroup".
+      iDestruct (txn_log_prefix with "Hlog Hloglb") as %Hprefix.
+      iPureIntro.
+      eapply apply_cmds_not_stuck; [apply Hprefix | by rewrite Hrsm].
+    }
+    iAssert (is_txn_pwrs γ gid ts pwrs ∗ ⌜dom pwrs ⊆ keys_all⌝)%I as "[#Hpwrs %Hdompwrs]".
+    { do 2 iNamed "Hgroup".
+      iDestruct (txn_log_prefix with "Hlog Hloglb") as %Hprefix.
+      iDestruct (txn_log_cpool_incl with "Hlog Hcpool") as %Hincl.
+      assert (Hin : CmdCommit ts pwrs ∈ cpool).
+      { rewrite /cpool_subsume_log Forall_forall in Hincl.
+        apply Hincl.
+        subst clog'.
+        eapply elem_of_prefix; last apply Hprefix.
+        set_solver.
+      }
+      iDestruct (big_sepS_elem_of with "Hsafecp") as "Hsafec"; first apply Hin.
+      iDestruct "Hsafec" as (wrs) "(_ & Hwrs & %Hpwrs & %Hgid & %Hvwrs)".
+      assert (Hdompwrs : dom pwrs ⊆ keys_all).
+      { rewrite Hpwrs wrs_group_keys_group_dom. set_solver. }
+      iFrame "Hwrs %".
+    }
+    do 2 iNamed "Hrp".
+    (* Agreement on the consistent and inconsistent logs. *)
+    iDestruct (replica_clog_agree with "Hclogprog Hclog") as %->.
+    iDestruct (replica_ilog_agree with "Hilogprog Hilog") as %->.
+    (* Update the consistent log. *)
+    iMod (replica_clog_update clog' with "Hclogprog Hclog") as "[Hclogprog Hclog]".
+    rewrite /not_stuck apply_cmds_snoc /= in Hns.
+    set st := LocalState _ _ _ _ _ _ in Hrsm.
+    (* Re-establish the RSM predicate. This will compute to the right form along
+    the way in each branch. *)
+    assert (Hrsm' : execute_cmds (merge_clog_ilog clog' ilog) = execute_commit st ts pwrs).
+    { rewrite merge_clog_ilog_snoc_clog; last apply Hpos.
+      by rewrite execute_cmds_snoc Hrsm.
+    }
+    iFrame "Hclogprog Hilogprog Hgroup".
+    unshelve epose proof (execute_cmds_apply_cmds clog ilog cm histm _) as Happly.
+    { by eauto. }
+    rewrite /apply_commit Happly in Hns.
+    subst st.
+    rewrite /execute_commit in Hrsm'.
+    destruct (cm !! ts) as [b |] eqn:Hcm.
+    { (* Case: Txn [ts] already finalized. Contradiction for aborted; no-op for committed. *)
+      destruct b; last done.
+      by iFrame "∗ # %".
+    }
+    (* Case: Txn [ts] not finalized. *)
+    (* Obtain facts about domain of the timestamp maps. *)
+    pose proof (map_Forall2_dom_L _ _ _ Hlenkvd) as Hdomsptsm.
+    symmetry in Hdomsptsm. rewrite Hdomkvdm in Hdomsptsm.
+    pose proof (map_Forall2_dom_L _ _ _ Hsptsmlk) as Hdomptsm.
+    symmetry in Hdomptsm. rewrite Hdomsptsm in Hdomptsm.
+    destruct (cpm !! ts) as [pwrs' |] eqn:Hcpm.
+    { (* Case: Txn [ts] prepared. *)      
+      (* Extend history, set commit map to true, reset currently prepared map and release locks. *)
+      iDestruct (big_sepM_delete _ _ ts with "Hsafep") as "[Hsafepwrs' Hsafep']".
+      { apply Hcpm. }
+      (* Agree on [pwrs] and [pwrs']. *)
+      iDestruct (safe_txn_pwrs_impl_is_txn_pwrs with "Hsafepwrs'") as "Hpwrs'".
+      iDestruct (txn_pwrs_agree with "Hpwrs Hpwrs'") as %->.
+      iClear "Hsafep".
+      set cm' := insert _ _ cm in Hrsm'.
+      set histm' := multiwrite _ _ _ in Hrsm'.
+      set cpm' := delete _ cpm in Hrsm'.
+      set ptsm' := release _ ptsm in Hrsm'.
+      iAssert (group_aborted_if_validated γ gid kvdm histm' ptsm')%I as "#Hgabt'".
+      { iIntros (k t).
+        destruct (decide (k ∈ dom pwrs)) as [Hin | Hnotin]; last first.
+        { rewrite multiwrite_unmodified; last by apply not_elem_of_dom.
+          by rewrite release_unmodified; last by apply not_elem_of_dom.
+        }
+        assert (is_Some (kvdm !! k)) as [vl Hvl].
+        { rewrite -elem_of_dom Hdomkvdm. clear -Hin Hdompwrs. set_solver. }
+        apply elem_of_dom in Hin as Hv.
+        destruct Hv as [v Hv].
+        pose proof (execute_cmds_dom_histm Hrsm) as Hdomhistm.
+        assert (is_Some (histm !! k)) as [h Hh].
+        { rewrite -elem_of_dom Hdomhistm. clear -Hin Hdompwrs. set_solver. }
+        rewrite (multiwrite_modified Hv Hh).
+        rewrite release_modified; last first.
+        { rewrite Hdomptsm. clear -Hin Hdompwrs. set_solver. }
+        { apply Hin. }
+        rewrite Hvl.
+        destruct (vl !! t) as [b |] eqn:Hvlt; last done.
+        destruct b; last done.
+        case_decide as Ht; last done.
+        destruct Ht as (Hgelen & Hnz).
+        assert (is_Some (ptsm !! k)) as [pts Hpts].
+        { rewrite -elem_of_dom Hdomptsm. clear -Hin Hdompwrs. set_solver. }
+        iSpecialize ("Hgabt" $! k t).
+        rewrite Hvl Hh Hpts Hvlt.
+        case_decide as Ht; first done.
+        exfalso.
+        apply Classical_Prop.not_and_or in Ht.
+        destruct Ht as [Hltlen | Ht].
+        { rewrite Nat.nle_gt in Hltlen.
+          clear -Hgelen Hltlen.
+          rewrite length_app /= in Hgelen.
+          pose proof (last_extend_length_ge ts h) as Hlen.
+          lia.
+        }
+        apply dec_stable in Ht. subst t.
+        (* Prove that [k] must be locked by [ts] (i.e., [ts = pts]. *)
+        specialize (Hpil _ _ _ Hcpm Hin).
+        rewrite Hpil in Hpts. inv Hpts.
+        pose proof (execute_cmds_hist_not_nil Hrsm) as Hnnil.
+        specialize (Hnnil _ _ Hh). simpl in Hnnil.
+        pose proof (last_extend_length_ge_n pts h Hnnil) as Hlen.
+        rewrite length_app /= in Hgelen.
+        clear -Hgelen Hlen. lia.
+      }
+      iFrame "∗ # %".
+      iPureIntro.
+      split.
+      { rewrite dom_insert_L dom_delete_L. clear -Hvtss.
+        rewrite -union_assoc union_comm -union_assoc difference_union_L.
+        set_solver.
+      }
+      split.
+      { rewrite map_Forall2_forall.
+        split; last by rewrite release_dom Hdomsptsm Hdomptsm.
+        intros k spts pts Hspts Hpts Hnz.
+        destruct (decide (k ∈ dom pwrs)) as [Hin | Hnotin]; last first.
+        { rewrite release_unmodified in Hpts; last by apply not_elem_of_dom.
+          apply (map_Forall2_lookup_Some _ _ _ _ _ _ Hspts Hpts Hsptsmlk Hnz).
+        }
+        rewrite release_modified in Hpts; last first.
+        { rewrite Hdomptsm. clear -Hin Hdompwrs. set_solver. }
+        { apply Hin. }
+        inv Hpts.
+      }
+      split.
+      { by apply prepared_impl_locked_inv_release. }
+      { rewrite lookup_delete_None. by right. }
+    }
+    (* Case: Txn [ts] not prepared. Extend history and set commit map. *)
+    set cm' := insert _ _ cm in Hrsm'.
+    set histm' := multiwrite _ _ _ in Hrsm'.
+    iAssert (group_aborted_if_validated γ gid kvdm histm' ptsm)%I as "#Hgabt'".
+    { iIntros (k t).
+      destruct (decide (k ∈ dom pwrs)) as [Hin | Hnotin]; last first.
+      { by rewrite multiwrite_unmodified; last by apply not_elem_of_dom. }
+      assert (is_Some (kvdm !! k)) as [vl Hvl].
+      { rewrite -elem_of_dom Hdomkvdm. clear -Hin Hdompwrs. set_solver. }
+      assert (is_Some (ptsm !! k)) as [pts Hpts].
+      { rewrite -elem_of_dom Hdomptsm. clear -Hin Hdompwrs. set_solver. }
+      rewrite Hvl Hpts.
+      apply elem_of_dom in Hin as Hv.
+      destruct Hv as [v Hv].
+      pose proof (execute_cmds_dom_histm Hrsm) as Hdomhistm.
+      assert (is_Some (histm !! k)) as [h Hh].
+      { rewrite -elem_of_dom Hdomhistm. clear -Hin Hdompwrs. set_solver. }
+      rewrite (multiwrite_modified Hv Hh).
+      destruct (vl !! t) as [b |] eqn:Hvlt; last done.
+      destruct b; last done.
+      case_decide as Ht; last done.
+      destruct Ht as [Hgelen Hnepts].
+      iSpecialize ("Hgabt" $! k t).
+      rewrite Hvl Hpts Hh Hvlt.
+      case_decide as Ht; first done.
+      exfalso.
+      apply Classical_Prop.not_and_or in Ht.
+      destruct Ht as [Hltlen | ?]; last done.
+      rewrite Nat.nle_gt in Hltlen.
+      clear -Hgelen Hltlen.
+      rewrite length_app /= in Hgelen.
+      pose proof (last_extend_length_ge ts h) as Hlen.
+      lia.
+    }
+    iFrame "∗ # %".
+    iPureIntro.
+    rewrite dom_insert_L.
+    clear -Hvtss. set_solver.
+  Qed.
+
+End execute_commit.
